abstract soundness derived

MultiScalarMul_Abstract.ec
@@ -7,10 +7,10 @@ require import BitEncoding StdBigop Bigalg.
 (*---*) import Bigint BIA.
 
 
-
-type R.                         (* quotient of points by unique repr, and subset of points on the curve *)
+(* unique representation of points on the curve *)
+type R.                         
+(* non-unique representation of points (not nec. on the curve) *)
 type F.
-type bits = bool list.
 
 op xof : R -> F.
 op yof : R -> F.
@@ -40,21 +40,51 @@ axiom op_id' (x : R) : idR +++ x = x.
 axiom op_inv (a : R) :  a +++ -a = idR. 
 
 axiom qiqq (i b : int) b0 :  (i + b) *** b0 = i *** b0 +++ b *** b0.
+axiom qiqq2 (i b : int) b0 :  (i * b) *** b0 = i *** (b *** b0).
+axiom qiqq3 (i : int) b0 :  (- i) *** b0 = - (i *** b0).
 axiom muldistR1 (a : R) : 1 *** a = a.
 axiom muldistR0 (a : R) : 0 *** a = idR. 
 axiom iteriZH : forall z, z *** idR = idR.
 axiom muldistR   : forall (a : int), forall (b c : R),   a *** (b +++ c) = a *** b +++ a *** c.
+
+
+
+lemma nosmt addass (a b c : int) : a + (b + c) = (a + b) + c.    by smt(). qed.
+lemma nosmt muldist (a b c : int) : a * (b + c) = a * b + a * c. by smt(). qed.
+lemma nosmt eqsym ['a] (a b : 'a) : a = b => b = a.              by smt(). qed.
+
+lemma kik  (a b c d : R) :  a +++ b +++ (c +++ d) = a +++ c +++ (b +++ d). 
+ by smt(op_assoc op_comm). qed.
+     
+lemma qiq : forall a, 0 <= a => forall (c : int), forall (b : R),
+   a *** b +++ c *** b = (a + c) *** b.
+apply natind. progress. smt.
+progress. rewrite qiqq. auto.
+have ->: (n + 1 + c) = ((n + c) + 1). smt().
+rewrite qiqq. 
+rewrite - H0. smt().    
+smt(op_comm op_assoc).
+qed.    
+
     
 op T : int.
 op l : int.
 op w : int.
+
+op onCurve : F -> bool.
+op idF     : F -> bool.
+op embed   : F -> R.
+
 axiom w_pos : 0 < w.
 axiom l_pos : 0 < l.
 axiom T_pos : 0 < T.
 
+module type OutCalls = {
+  proc getU() : F
+  proc getT(P : int -> R, v : R) : int -> int -> R
+}.
 
-
-module MultiScalarMul = {
+module MultiScalarMul(O : OutCalls) = {
 
   proc helper(acc : int, table : int -> int-> int, ic : int, P : int -> int, s : int -> int -> int, U : int) = {
       var jc, aux, vahe;
@@ -98,12 +128,13 @@ module MultiScalarMul = {
 
 
   proc multiScalarMulR(P : int -> R, s : int -> int -> int, U : R) = {
-    var u, v, acc, aux, result : R;
+    var v, acc, aux, result : R;
     var table : int -> int -> R;
     var ic, jc, cnt : int;
 
+   
     v     <- (2 ^ w - 1) *** U;
-    table <- fun (j i : int) => (i *** (P j)) +++ - v;
+    table <@ O.getT(P, v);
     acc   <- l *** U;
 
     ic <- 0;
@@ -148,7 +179,7 @@ module MultiScalarMul = {
     flag  <- true;
     flagaux <- true;
     v     <- (2 ^ w - 1) *** U;
-    table <- fun (j i : int) => (i *** (P j)) +++ - v;
+    table <@ O.getT(P, v);
     acc   <- l *** U;
 
     ic <- 0;
@@ -163,6 +194,25 @@ module MultiScalarMul = {
     return (flag, result);
   }
 
+  proc multiScalarMul(P : int -> R, s : int -> int -> int) = {
+    var u_cand : F;
+    var flag : bool;
+    var result;
+
+    u_cand <@ O.getU();
+    flag <- ! idF u_cand && onCurve u_cand;
+
+    if(flag = true) {
+      result <@ multiScalarMulI(P,s,embed u_cand);
+    } else{
+      result <- (false, witness);    
+    } 
+
+
+    return result;
+  }
+
+
 }.
 
 
@@ -176,110 +226,72 @@ op multiScalarMulR  (s : int -> int -> int) (P : int -> R)
           acc2 +++ (2 ^ (w * (T - 1 - i)) * s j i) *** (P j)) idR
         ) idR.
 
+section.
 
+declare module O <: OutCalls.
+
+declare axiom tableP parg varg : hoare [ O.getT : arg = (parg,varg)
+   ==> res = (fun (j i : int) =>  (i *** (parg j)) +++ - varg)  ].
+declare axiom getT_lossless : islossless O.getT.
 
 
 lemma helpereqs argacc argtable argic args  : 
- equiv [ MultiScalarMul.helperR ~ MultiScalarMul.helperI  : 
+ equiv [ MultiScalarMul(O).helperR ~ MultiScalarMul(O).helperI : 
   arg{2} = (argacc, argtable, argic, args) /\ ={acc,table,ic,s}
+       /\ (forall i j, table{1} i j <> idR)
      ==>  res{2}.`1 => (res{1} = res{2}.`2)].
 proc.
-while (={jc,acc,table,aux,s,ic} /\ (flag{2} => ={vahe})).
+while (={jc,acc,table,aux,s,ic} /\ (flag{2} => ={vahe})
+ /\ (forall i j, table{1} i j <> idR)).
  wp. skip. progress.
    have -> : vahe{1} = vahe{2}. smt().
 rewrite same_res. 
   smt().
-  admit. 
+  smt(). 
   smt().
   smt().
 wp. skip. progress. 
 qed.
 
-(* 
-1/ compute table externally
-2/ get U outside in a primitive way
-3/ ?
-
-
-
-
-*)
-
-lemma multieqs argP args argU  : 
- equiv [ MultiScalarMul.multiScalarMulR ~ MultiScalarMul.multiScalarMulI : 
-  arg{2} = (argP, args, argU) /\ ={P,s,U}
-     ==>  res{2}.`1 => (res{1} = res{2}.`2)].
-proc.
-wp.
-while ((flag{2} => ={table,acc,U,s}) /\ (flag{2} => flagaux{2}) /\ ={ic}  ).
-wp.   
-inline MultiScalarMul.helperR.
-inline MultiScalarMul.helperI.
-wp.   
-while ((flag{2} /\ flag0{2} => ={vahe, acc0,table0,aux0,s0,ic0}) /\ ={jc0}).
- wp. skip. progress.
-   have -> : vahe{1} = vahe{2}. smt().
-rewrite same_res. 
-  smt().
-  admit. 
-  smt().
-  smt().
-     smt().
-     smt().
-     smt().
-     smt().
-     smt().
-wp. 
-inline MultiScalarMul.doubleWtimes.
-wp.
-   while ((flag{2} => ={p}) /\ ={w,cnt0}). wp. skip. progress.
-   smt(). wp. skip. progress. 
-smt(). smt(). smt(). smt(). smt(). smt().
-   smt(). smt().  smt().
-wp. skip. progress.
-have -> :     acc_L = acc_R. smt(). auto.
-qed.
-
+    
    
-lemma helper_specR argcc argT argic args  : 
- hoare [ MultiScalarMul.helperR : arg = (argcc, argT, argic,  args) 
-     ==>  res = argcc +++  iteri l (fun j acc => acc +++ argT j (args j argic)) idR ].
+lemma helper_specR_ph argcc argT argic args  : 
+ phoare [ MultiScalarMul(O).helperR : arg = (argcc, argT, argic,  args) 
+     ==>  res = argcc +++  iteri l (fun j acc => acc +++ argT j (args j argic)) idR ] = 1%r.
 proc.
 while (0 <= jc 
  /\ jc <= l 
  /\ (acc, table, ic,  s) = (argcc, argT, argic, args) 
- /\ vahe = acc +++   iteri jc (fun j acc => acc +++ argT j (args j argic)) idR).
+ /\ vahe = acc +++   iteri jc (fun j acc => acc +++ argT j (args j argic)) idR) (l - jc).
+move => z.
 wp. skip. progress. smt(). smt(). rewrite iteriS. smt().
    simplify.
 smt(op_assoc).
+smt().   
    wp. skip. progress. smt(l_pos). 
 rewrite iteri0. auto.
 smt(op_id).
 smt().
+smt().
 qed.   
 
 
-lemma nosmt addass (a b c : int) : a + (b + c) = (a + b) + c.    by smt(). qed.
-lemma nosmt muldist (a b c : int) : a * (b + c) = a * b + a * c. by smt(). qed.
-lemma nosmt eqsym ['a] (a b : 'a) : a = b => b = a.              by smt(). qed.
-
-
-
-lemma kik  (a b c d : R) :  a +++ b +++ (c +++ d) = a +++ c +++ (b +++ d). 
- by smt(op_assoc op_comm). qed.
-
-     
-lemma qiq : forall a, 0 <= a => forall (c : int), forall (b : R),
-   a *** b +++ c *** b = (a + c) *** b.
-apply natind. progress. smt.
-progress. rewrite qiqq. auto.
-have ->: (n + 1 + c) = ((n + c) + 1). smt().
-rewrite qiqq. 
-rewrite - H0. smt().    
-smt(op_comm op_assoc).
+lemma helper_specR_total  : 
+ phoare [ MultiScalarMul(O).helperR : true ==>  true ] = 1%r.
+proc*.
+exists*  acc, table, ic, s.
+elim*. move => accV tableV icV sV.        
+call (helper_specR_ph accV tableV icV sV).
+auto.
 qed.    
 
 
+lemma helper_specR argcc argT argic args  : 
+ hoare [ MultiScalarMul(O).helperR : arg = (argcc, argT, argic,  args) 
+     ==>  res = argcc +++  iteri l (fun j acc => acc +++ argT j (args j argic)) idR ].
+conseq (helper_specR_ph argcc argT argic args).   
+progress.
+qed.   
 
 
 lemma iteriZ : forall (n : int), 0 <= n =>  forall (z : int) (f : int -> R), z *** (iteri n (fun i acc => acc +++ f i) idR)
@@ -311,7 +323,6 @@ smt (op_assoc op_comm).
 qed.     
 
 
-
 lemma iteriZZZ  : forall (n : int), 0 <= n => forall (z : R),
   (iteri n (fun i acc => acc +++ z) idR)
      = n *** z.
@@ -337,11 +348,13 @@ rewrite H0.
 rewrite qiqq. smt.
 qed.    
 
-lemma doublewtimes_spec argP argw :
- hoare [ MultiScalarMul.doubleWtimes : arg = (argP, argw) /\
-   0 <= argw  ==>  res = (2 ^ argw) *** argP  ].
+
+lemma doublewtimes_spec_ph argP argw :
+ phoare [ MultiScalarMul(O).doubleWtimes : arg = (argP, argw) /\
+   0 <= argw  ==>  res = (2 ^ argw) *** argP  ] = 1%r.
 proc. 
-   while (cnt <= w /\ 0 <= argw /\ 0 <= cnt /\ p = (2 ^ cnt) *** argP).
+   while (cnt <= w /\ 0 <= argw /\ 0 <= cnt /\ p = (2 ^ cnt) *** argP) (w - cnt).
+move => z.    
    wp.
    skip. progress. smt(). smt().
    rewrite qiq. smt.
@@ -349,32 +362,40 @@ proc.
    smt(@Int).
    congr.
    rewrite exprS. auto. auto.
-   wp. skip. progress. smt.
+   smt().
+   wp. skip. progress. smt. smt().
    smt(@Int).
 qed.
 
 
+lemma doublewtimes_spec argP argw :
+ hoare [ MultiScalarMul(O).doubleWtimes : arg = (argP, argw) /\
+   0 <= argw  ==>  res = (2 ^ argw) *** argP  ].
+conseq (doublewtimes_spec_ph argP argw).   
+qed.   
+
+
 lemma multiscalarR_spec argP args argU : 
- hoare [ MultiScalarMul.multiScalarMulR : 
+ hoare [ MultiScalarMul(O).multiScalarMulR : 
   arg = (argP, args, argU) 
      ==>  res = (multiScalarMulR  args argP)  ].
-proc. wp.   
-while (0 <= ic 
- /\ (2 ^ w - 1) *** U = v 
- /\ table = (fun (j i : int) =>  (i *** (P j)) +++ - v) 
- /\ ic <= T  
+proc. wp.
+while (0 <= ic
+ /\ (2 ^ w - 1) *** U = v
+ /\ table = (fun (j i : int) =>  (i *** (P j)) +++ - v)
+ /\ ic <= T
  /\ acc = ((iteri ic
             (fun i acc1 => acc1 +++
               (iteri l
-                 (fun j acc2 => acc2 +++ (2 ^ (w * (ic - 1 - i)) * s j i) *** (P j)) idR) 
+                 (fun j acc2 => acc2 +++ (2 ^ (w * (ic - 1 - i)) * s j i) *** (P j)) idR)
                  ) idR)) +++ l *** U).
-wp. 
+wp.
 ecall (helper_specR acc table ic s). simplify.
 wp.
 ecall (doublewtimes_spec acc w). skip. progress. smt(w_pos).
 smt(). smt().
-   rewrite muldistR. 
-rewrite iteriZ.           smt(). 
+   rewrite muldistR.
+rewrite iteriZ.           smt().
 simplify.
 have -> : iteri ic{hr}
   (fun (i : int) (acc0 : R) =>
@@ -387,60 +408,48 @@ have -> : iteri ic{hr}
      = iteri ic{hr}
   (fun (i : int) (acc0 : R) =>
      acc0 +++
-     
      iteri l
        (fun (j : int) (acc2 : R) =>
           acc2 +++ 2 ^ (w * (ic{hr}  - i )) * s{hr} j i *** P{hr} j) idR)
   idR.
-apply eq_iteri. 
-
+apply eq_iteri.
 progress.
-
 rewrite iteriZ. smt(l_pos). congr.
      apply eq_iteri. move => j acc.
      progress. congr.
       have ->: 2 ^ w *** (2 ^ (w * (ic{hr} - 1 - i)) * s{hr} j i *** P{hr} j)
                 = 2 ^ w * 2 ^ (w * (ic{hr} - 1 - i)) * s{hr} j i *** P{hr} j .
-  rewrite mulsc. smt. smt().                
+  rewrite mulsc. smt. smt().
         rewrite - exprD_nneg. smt(w_pos). smt(w_pos). smt().
-
 pose v := (2 ^ w - 1) *** U{hr}.
- 
 have -> : iteri l
   (fun (j : int) (acc0 : R) => acc0 +++ (s{hr} j ic{hr} *** P{hr} j +++ -v))
   idR = iteri l
-  (fun (j : int) (acc0 : R) => acc0 +++ (s{hr} j ic{hr} *** P{hr} j)) idR +++ 
+  (fun (j : int) (acc0 : R) => acc0 +++ (s{hr} j ic{hr} *** P{hr} j)) idR +++
      iteri l (fun (j : int) (acc0 : R) => acc0 +++ -v) idR.
-rewrite - iteriZZ. simplify. 
+rewrite - iteriZZ. simplify.
 smt(l_pos). apply eq_iteri.  progress. smt.
-simplify.  
-rewrite  iteriZZZ.            
-
+simplify.
+rewrite  iteriZZZ.
 simplify. smt(l_pos).
 rewrite kik .
-   
 have ->: (2 ^ w *** (l *** U{hr}) +++ l *** -v) = l *** U{hr}.
     rewrite /v.
   rewrite  mulsc. smt.
-  have ->: - (2 ^ w - 1) *** U{hr} = (- (2 ^ w - 1)) *** U{hr}. admit.
-  rewrite (mulsc ). smt(l_pos).
-  rewrite qiq. smt.
- smt(@Int).
-  
+  have -> : l *** - (2 ^ w - 1) *** U{hr}
+    = (l * - (2 ^ w - 1)) *** U{hr}. rewrite  qiqq2.  rewrite qiqq3. auto.
+   rewrite - qiqq. congr. smt().
 
-rewrite iteriS. 
-
-smt(). simplify. 
-
+rewrite iteriS.
+smt(). simplify.
 have ->: 2 ^ 0 = 1. smt(@Int).
-smt().     
-wp. skip. progress. smt(T_pos). 
-   
+smt().
+wp.
+ecall (tableP P v). wp. skip. progress. smt(T_pos).
 rewrite iteri0. auto. smt.
 rewrite /multiScalarMulInt.
 have -> : ic0 = T. smt().
 simplify.
-
   have ->: iteri T
   (fun (i : int) (acc1 : R) =>
      acc1 +++
@@ -461,3 +470,108 @@ rewrite op_inv.
   rewrite /multiScalarMulR.
 auto.
 qed.
+
+
+lemma multiscalarR_spec_ph argP args argU : 
+ phoare [ MultiScalarMul(O).multiScalarMulR : 
+  arg = (argP, args, argU) 
+     ==>  res = (multiScalarMulR  args argP)  ] = 1%r.
+phoare split ! 1%r 0%r. auto.
+   proc. wp.
+while true (T - ic). progress.
+wp.
+exists* acc, table, ic, s.
+elim*. move => accV tableV icV sV.
+call helper_specR_total.   
+call (_: arg = (accV, Top.w) ==> true).
+proc*. call (doublewtimes_spec_ph accV Top.w).
+skip. progress. smt(w_pos). skip.
+progress.
+smt().
+wp. call (_:true). apply getT_lossless. 
+wp. skip. progress. smt().
+hoare. simplify.   
+apply multiscalarR_spec.
+qed.
+
+lemma multieqs argP args argU  :
+ equiv [ MultiScalarMul(O).multiScalarMulR 
+        ~ MultiScalarMul(O).multiScalarMulI :
+  arg{2} = (argP, args, argU) /\ ={P,s,U} /\ ={glob O}
+     ==>  res{2}.`1 => (res{1} = res{2}.`2)].
+proc.
+wp.
+while ((flag{2} => ={table,acc,U,s}) /\ (flag{2} => flagaux{2}) /\ ={ic}  ).
+wp.
+inline MultiScalarMul(O).helperR.
+inline MultiScalarMul(O).helperI.
+wp.
+while ((flag{2} /\ flag0{2} => ={vahe, acc0,table0,aux0,s0,ic0}) /\ ={jc0}).
+ wp. skip. progress.
+   have -> : vahe{1} = vahe{2}. smt().
+rewrite same_res.
+  smt().
+  admit.
+  smt().
+  smt().
+     smt().
+     smt().
+     smt().
+     smt().
+     smt().
+wp.
+inline MultiScalarMul(O).doubleWtimes.
+wp.
+   while ((flag{2} => ={p}) /\ ={w,cnt0}). wp. skip. progress.
+   smt(). wp. skip. progress.
+smt(). smt(). smt(). smt(). smt(). smt().
+   smt(). smt().  smt().
+wp. call (_:true). wp. skip. progress.
+have -> :     acc_L = acc_R. smt(). auto.
+qed.
+
+lemma multiscalarI_spec_ph argP args  argU : 
+ phoare [ MultiScalarMul(O).multiScalarMulI : 
+  arg = (argP, args, argU) 
+     ==>  res.`1 => res.`2 = (multiScalarMulR  args argP)  ] = 1%r.
+proof.
+bypr.
+progress.
+have ih: 1%r = Pr[MultiScalarMul(O).multiScalarMulR(P{m}, s{m}, U{m}) @ &m 
+  : res = multiScalarMulR args argP].
+byphoare (_: arg = (argP, args, argU) ==> _).
+conseq (multiscalarR_spec_ph argP args argU). smt(). auto.
+have : Pr[MultiScalarMul(O).multiScalarMulI(P{m}, s{m}, U{m}) @ &m :
+   res.`1 => res.`2 = multiScalarMulR args argP] >=
+Pr[MultiScalarMul(O).multiScalarMulR(P{m}, s{m}, U{m}) @ &m :
+   res = multiScalarMulR args argP].
+byequiv (_: _ ==> res{2}.`1 => res{2}.`2 = res{1} ).
+proc*.
+ecall (multieqs argP args argU).
+skip. progress. smt(). smt(). smt(). smt().
+auto.
+smt().
+smt.
+qed.
+
+lemma multiscalarI_spec_h argP args  argU : 
+ hoare [ MultiScalarMul(O).multiScalarMulI : 
+  arg = (argP, args, argU) 
+     ==>  res.`1 => res.`2 = (multiScalarMulR  args argP)  ] .
+conseq (multiscalarI_spec_ph argP args argU).
+qed.   
+
+
+lemma multiscalar_spec_h argP args : 
+ hoare [ MultiScalarMul(O).multiScalarMul : 
+  arg = (argP, args) 
+     ==>  res.`1 => res.`2 = (multiScalarMulR  args argP)  ] .
+proc.
+seq 1 : #pre.
+call (_: true). auto.
+sp. if.
+  ecall (multiscalarI_spec_h P s (embed u_cand)).
+   skip. progress.
+wp. skip.
+smt().
+qed.   
